src/Utility.v
@@ -11,17 +11,21 @@ Global Unset Universe Minimization ToSet.
 
 Local Open Scope Z_scope.
 
+(* when we don't need any operators, we just use tuples of bytes: *)
+Section ByteTuples.
+  Context {byte: word 8}.
+  Definition w8  := tuple byte 1.
+  Definition w16 := tuple byte 2.
+  Definition w32 := tuple byte 4.
+  Definition w64 := tuple byte 8.
+End ByteTuples.
+
 (* Meaning of MachineInt: an integer big enough to hold an integer of a RISCV machine,
    no matter whether it's a 32-bit or 64-bit machine. *)
 Definition MachineInt := Z.
 
 Class MachineWidth(t: Type) := {
-  byte: word 8;
-
-  w8  := tuple byte 1;
-  w16 := tuple byte 2;
-  w32 := tuple byte 4;
-  w64 := tuple byte 8;
+  byte :> word 8;
 
   (* arithmetic operations (inherited from wegral in Haskell) *)
   add: t -> t -> t;
@@ -86,48 +90,6 @@ Class MachineWidth(t: Type) := {
 
   (* additional conversions: *)
   ZToReg: Z -> t;
-
-  (* properties of operations: *)
-  (* TODO list separately to make them more discoverable by "Search" *)
-  regRing: @ring_theory t (ZToReg 0) (ZToReg 1) add mul sub negate (@eq t);
-  ZToReg_morphism: @ring_morph t (ZToReg 0) (ZToReg 1) add mul sub negate (@eq t)
-                               Z 0 1 Z.add Z.mul Z.sub Z.opp Z.eqb ZToReg;
-
-  reg_eqb_spec: forall a b, reg_eqb a b = true <-> a = b;
-
-  regToZ_signed_bounds: forall a, - 2 ^ (XLEN - 1) <= regToZ_signed a < 2 ^ (XLEN - 1);
-  regToZ_unsigned_bounds: forall a, 0 <= regToZ_unsigned a < 2 ^ XLEN;
-
-  add_def_signed: forall a b, add a b = ZToReg (regToZ_signed a + regToZ_signed b);
-  sub_def_signed: forall a b, sub a b = ZToReg (regToZ_signed a - regToZ_signed b);
-  mul_def_signed: forall a b, mul a b = ZToReg (regToZ_signed a * regToZ_signed b);
-
-  regToZ_ZToReg_signed: forall n : Z,
-      - 2 ^ (XLEN - 1) <= n < 2 ^ (XLEN - 1) ->
-      regToZ_signed (ZToReg n) = n;
-  regToZ_ZToReg_unsigned_mod: forall n : Z, regToZ_unsigned (ZToReg n) = n mod 2 ^ XLEN;
-
-  ZToReg_regToZ_unsigned: forall a: t, ZToReg (regToZ_unsigned a) = a;
-  ZToReg_regToZ_signed: forall a: t, ZToReg (regToZ_signed a) = a;
-
-  XLEN_lbound: 8 <= XLEN;
-
-  (* Note: There are 3 ways to define div and mod:
-     - truncate division (aka round towards zero, aka "T"), define mod as remainder wrt division
-       Defined in Coq in Module ZDivTrunc and available as Z.quot and Z.rem.
-       That's also what RISC-V does, according to
-       https://github.com/riscv/riscv-isa-manual/commit/3de73dedf7822bf35f0fa603e400c4f25c99b6d9
-     - floor division (aka "F"), define mod as remainder wrt division
-       Defined in Coq in Module ZDivFloor and available as Z.div and Z.modulo.
-     - Euclidian division, where the remainder never is negative (aka "E"):
-       forall a b, b<>0 -> exists r q, a = b*q+r /\ 0 < r < |b|
-       Defined in Coq in Module ZDivEucl.
-     Note: The corner cases (division by 0, overflow) are handled in ExecuteM.
-  *)
-  div_def : forall a b, div  a b = ZToReg (Z.quot (regToZ_signed   a) (regToZ_signed   b));
-  rem_def : forall a b, rem  a b = ZToReg (Z.rem  (regToZ_signed   a) (regToZ_signed   b));
-  divu_def: forall a b, divu a b = ZToReg (Z.quot (regToZ_unsigned a) (regToZ_unsigned b));
-  remu_def: forall a b, remu a b = ZToReg (Z.rem  (regToZ_unsigned a) (regToZ_unsigned b));
 }.
 
 Notation fromImm := (@ZToReg _ _) (only parsing).
@@ -140,116 +102,6 @@ Section Derived.
   Definition XLEN_in_bytes: Z := XLEN / 8.
 
   Definition lnot(x: t): t := xor x maxUnsigned.
-
-  Lemma reg_eqb_true: forall a b, reg_eqb a b = true -> a = b.
-  Proof. apply reg_eqb_spec. Qed.
-
-  Lemma reg_eqb_eq: forall a b, a = b -> reg_eqb a b = true.
-  Proof. apply reg_eqb_spec. Qed.
-
-  Lemma reg_eqb_false: forall a b, reg_eqb a b = false -> a <> b.
-  Proof.
-    intros. intro. rewrite reg_eqb_eq in H; congruence.
-  Qed.
-
-  Lemma reg_eqb_ne: forall a b, a <> b -> reg_eqb a b = false.
-  Proof.
-    intros. destruct (reg_eqb a b) eqn: E; try congruence.
-    exfalso. apply H. apply reg_eqb_true in E. assumption.
-  Qed.
-
-  Lemma regToZ_ZToReg_unsigned: forall n : Z,
-      0 <= n < 2 ^ XLEN ->
-      regToZ_unsigned (ZToReg n) = n.
-  Proof.
-    intros.
-    rewrite regToZ_ZToReg_unsigned_mod.
-    apply Z.mod_small.
-    assumption.
-  Qed.
-
-  Lemma add_def_unsigned: forall a b, add a b = ZToReg (regToZ_unsigned a + regToZ_unsigned b).
-  Proof.
-    intros.
-    rewrite ZToReg_morphism.(morph_add). rewrite? ZToReg_regToZ_unsigned.
-    reflexivity.
-  Qed.
-
-  Lemma sub_def_unsigned: forall a b, sub a b = ZToReg (regToZ_unsigned a - regToZ_unsigned b).
-  Proof.
-    intros.
-    rewrite ZToReg_morphism.(morph_sub). rewrite? ZToReg_regToZ_unsigned.
-    reflexivity.
-  Qed.
-
-  Lemma mul_def_unsigned: forall a b, mul a b = ZToReg (regToZ_unsigned a * regToZ_unsigned b).
-  Proof.
-    intros.
-    rewrite ZToReg_morphism.(morph_mul). rewrite? ZToReg_regToZ_unsigned.
-    reflexivity.
-  Qed.
-
-  Lemma ZToReg_inj_unsigned: forall a b,
-      0 <= a < 2 ^ XLEN ->
-      0 <= b < 2 ^ XLEN ->
-      ZToReg a = ZToReg b ->
-      a = b.
-  Proof.
-    intros.
-    (* Check (ZToReg_morphism.(morph_eq)). the wrong way *)
-  Abort.
-
-  Lemma pow2_sz_4: 4 < 2 ^ XLEN.
-  Proof.
-    pose proof XLEN_lbound.
-    change 4 with (2 ^ 2).
-    apply Z.pow_lt_mono_r; omega.
-  Qed.
-
-  Lemma regToZ_unsigned_eq: forall (a b: t), regToZ_unsigned a = regToZ_unsigned b -> a = b.
-  Proof.
-    intros.
-    rewrite <- (ZToReg_regToZ_unsigned a).
-    rewrite <- (ZToReg_regToZ_unsigned b).
-    congruence.
-  Qed.
-
-  Lemma regToZ_unsigned_ne: forall (a b: t), regToZ_unsigned a <> regToZ_unsigned b -> a <> b.
-  Proof.
-    intros.
-    intro C.
-    subst b.
-    apply H.
-    reflexivity.
-  Qed.
-
-  Lemma ne_regToZ_unsigned: forall (a b: t),
-      a <> b -> regToZ_unsigned a <> regToZ_unsigned b.
-  Proof.
-    intros.
-    intro C.
-    apply H.
-    apply regToZ_unsigned_eq.
-    assumption.
-  Qed.
-
-  Lemma regToZ_unsigned_one: regToZ_unsigned (ZToReg 1) = 1.
-  Proof.
-    intros.
-    apply regToZ_ZToReg_unsigned. pose proof pow2_sz_4. omega.
-  Qed.
-
-  Lemma regToZ_unsigned_two: regToZ_unsigned (ZToReg 2) = 2.
-  Proof.
-    intros.
-    apply regToZ_ZToReg_unsigned. pose proof pow2_sz_4. omega.
-  Qed.
-
-  Lemma regToZ_unsigned_four: regToZ_unsigned (ZToReg 4) = 4.
-  Proof.
-    intros.
-    apply regToZ_ZToReg_unsigned. pose proof pow2_sz_4. omega.
-  Qed.
 
 End Derived.
 
